src/Step.v
@@ -9,138 +9,135 @@ Require Import Subst.
 Require Maps.
 Import Maps.Notations.
 
+Reserved Notation "x ->> y" (at level 70, no associativity).
+
 Inductive step : expr -> expr -> Prop := 
   | ST_App_Fun : 
       ∀ (x : string) (t : type) (e e' v : expr),
       value v -> 
       substitution v x e e' ->
-      step (E_App (E_Fun x t e) v) e'
+      (E_App (E_Fun x t e) v) ->> e'
   | ST_App_Left : 
       ∀ (e1 e1' e2 : expr),
-      step e1 e1' ->
-      step (E_App e1 e2) (E_App e1' e2)
+      e1 ->> e1' ->
+      (E_App e1 e2) ->> (E_App e1' e2)
   | ST_App_Right : 
       ∀ (v1 e2 e2' : expr),
       value v1 ->
-      step e2 e2' ->
-      step (E_App v1 e2) (E_App v1 e2')
+      e2 ->> e2' ->
+      (E_App v1 e2) ->> (E_App v1 e2')
   | ST_If_True : 
       ∀ (e1 e2 : expr),
-      step (E_If E_True e1 e2) e1
+      (E_If E_True e1 e2) ->> e1
   | ST_If_False : 
       ∀ (e1 e2 : expr),
-      step (E_If E_False e1 e2) e2
+      (E_If E_False e1 e2) ->> e2
   | ST_If : 
       ∀ (e1 e1' e2 e3 : expr),
-      step e1 e1' ->
-      step (E_If e1 e2 e3) (E_If e1' e2 e3)
+      e1 ->> e1' ->
+      (E_If e1 e2 e3) ->> (E_If e1' e2 e3)
   | ST_Let_Left : 
       ∀ (x : string) (e1 e1' e2 : expr),
-      step e1 e1' ->
-      step (E_Let x e1 e2) (E_Let x e1' e2)
+      e1 ->> e1' ->
+      (E_Let x e1 e2) ->> (E_Let x e1' e2)
   | ST_Let_Right : 
       ∀ (x : string) (v1 e2 e2' : expr),
       value v1 ->
       substitution v1 x e2 e2' ->
-      step (E_Let x v1 e2) e2'
+      (E_Let x v1 e2) ->> e2'
   | ST_Minus_Left :  
       ∀ (e1 e1' e2 : expr),
-      step e1 e1' ->
-      step (E_Minus e1 e2) (E_Minus e1' e2)
+      e1 ->> e1' ->
+      (E_Minus e1 e2) ->> (E_Minus e1' e2)
   | ST_Minus_Right :  
       ∀ (v1 e2 e2' : expr),
       value v1 ->
-      step e2 e2' ->
-      step (E_Minus v1 e2) (E_Minus v1 e2')
+      e2 ->> e2' ->
+      (E_Minus v1 e2) ->> (E_Minus v1 e2')
   | ST_Minus_Num : 
       ∀ (z1 z2 : Z),
-      step 
-          (E_Minus (E_Num z1) (E_Num z2))
-          (E_Num (z1 - z2))
+      (E_Minus (E_Num z1) (E_Num z2)) ->> (E_Num (z1 - z2))
 
   | ST_Eq_Left :  
       ∀ (e1 e1' e2 : expr),
-      step e1 e1' ->
-      step (E_Eq e1 e2) (E_Eq e1' e2)
+      e1 ->> e1' ->
+      (E_Eq e1 e2) ->> (E_Eq e1' e2)
   | ST_Eq_Right :  
       ∀ (v1 e2 e2' : expr),
       value v1 ->
-      step e2 e2' ->
-      step (E_Eq v1 e2) (E_Eq v1 e2')
+      e2 ->> e2' ->
+      (E_Eq v1 e2) ->> (E_Eq v1 e2')
   | ST_Eq_Num_Eq : 
       ∀ (z : Z),
-      step 
-          (E_Eq (E_Num z) (E_Num z))
-          (E_True)
+      (E_Eq (E_Num z) (E_Num z)) ->> (E_True)
   | ST_Eq_Num_Neq : 
       ∀ (z1 z2 : Z),
       z1 <> z2 ->
-      step 
-          (E_Eq (E_Num z1) (E_Num z2))
-          (E_False)
+      (E_Eq (E_Num z1) (E_Num z2)) ->> (E_False)
 
 
   | ST_Pair_Left :  
       ∀ (e1 e1' e2 : expr),
-      step e1 e1' ->
-      step (E_Pair e1 e2) (E_Pair e1' e2)
+      e1 ->> e1' ->
+      (E_Pair e1 e2) ->> (E_Pair e1' e2)
   | ST_Pair_Right :  
       ∀ (v1 e2 e2' : expr),
       value v1 ->
-      step e2 e2' ->
-      step (E_Pair v1 e2) (E_Pair v1 e2')
+      e2 ->> e2' ->
+      (E_Pair v1 e2) ->> (E_Pair v1 e2')
   | ST_First :  
       ∀ (e e' : expr),
-      step e e' ->
-      step (E_First e) (E_First e')
+      e ->> e' ->
+      (E_First e) ->> (E_First e')
   | ST_Second :  
       ∀ (e e' : expr),
-      step e e' ->
-      step (E_Second e) (E_Second e')
+      e ->> e' ->
+      (E_Second e) ->> (E_Second e')
   | ST_First_Pair :  
       ∀ (v₁ v₂ : expr),
       value v₁ -> 
       value v₂ ->
-      step (E_First (E_Pair v₁ v₂)) v₁
+      (E_First (E_Pair v₁ v₂)) ->> v₁
   | ST_Second_Pair :  
       ∀ (v₁ v₂ : expr),
       value v₁ -> 
       value v₂ ->
-      step (E_Second (E_Pair v₁ v₂)) v₂
+      (E_Second (E_Pair v₁ v₂)) ->> v₂
   
   | ST_Record_Tail : 
       ∀ x e tail tail', 
-      step tail tail' -> 
-      step (E_Record_Cons x e tail) (E_Record_Cons x e tail')
+      tail ->> tail' -> 
+      (E_Record_Cons x e tail) ->> (E_Record_Cons x e tail')
   
   | ST_Record : 
       ∀ x e e' tail,
       value tail -> 
-      step e e' -> 
-      step (E_Record_Cons x e tail) (E_Record_Cons x e' tail)
+      e ->> e' -> 
+      (E_Record_Cons x e tail) ->> (E_Record_Cons x e' tail)
   
   | ST_Access : 
       ∀ x e e',
-      step e e' ->
-      step (E_Record_Access e x) (E_Record_Access e' x)
+      e ->> e' ->
+      (E_Record_Access e x) ->> (E_Record_Access e' x)
 
   | ST_Access_Value : 
       ∀ x e v,
       value e -> 
       lookup_val_record x e = Some v ->
-      step (E_Record_Access e x) v
+      (E_Record_Access e x) ->> v
 
   | ST_Fix :
       ∀ (e e': expr),
-      step e e' ->
-      step (E_Fix e) (E_Fix e')
+      e ->> e' ->
+      (E_Fix e) ->> (E_Fix e')
   
   | ST_Fix_Fun :
       ∀ x t e e',
       substitution (E_Fix (E_Fun x t e)) x e e' ->
-      step 
-        (E_Fix (E_Fun x t e)) 
-        e'
+      (E_Fix (E_Fun x t e)) ->> e'
+
+where 
+    "x ->> y" := (step x y)
 .
 
 Hint Constructors step : local_hints.
@@ -150,7 +147,7 @@ Hint Constructors step : local_hints.
 Local Lemma not_value: 
   ∀ e e',
   value e -> 
-  ~ step e e'.
+  ~ e ->> e'.
 Proof.
   induction e; intros e' H_val H_contra;
   try (inversion H_val; inversion H_contra; fail).
