src/Multi.v
@@ -1,0 +1,157 @@
+From Coq Require Import Unicode.Utf8.
+From Coq Require Import Relation_Definitions.
+Require Import Syntax.
+Require Import Step.
+Require Import Subst.
+Require Import Hints.
+Require Import Closed.
+Local Open Scope Z_scope.
+Require Import ZArith.
+Require Import Lia.
+Require Import String.
+
+
+Reserved Notation "e1 ->>* e2" (at level 70, no associativity) .
+
+Inductive multistep : expr -> expr -> Prop :=
+  | multistep_step : 
+      ∀ e1 e2, 
+      e1 ->> e2 -> 
+      e1 ->>* e2 
+  | multistep_refl : 
+      ∀ e, 
+      e ->>* e 
+  | multistep_trans :
+      ∀ x y z,
+      x ->>* y -> 
+      y ->>* z -> 
+      x ->>* z 
+  where "e1 ->>* e2" := (multistep e1 e2)
+  .
+
+Hint Constructors multistep : local_hints.
+
+Lemma multistep_step_ : ∀ e1 e2, e1 ->> e2 -> e1 ->>* e2.
+Proof.
+  eauto with local_hints.
+  Show Proof.
+Qed.
+
+
+Example multistep_if :
+  <{if 1 == 2 then 3 else 0}> ->>* <{0}>.
+Proof.
+  eauto 6 with zarith local_hints.
+Qed.
+
+Definition eq := "eq"%string.
+Definition m := "m"%string.
+Definition n := "n"%string.
+
+Definition inner_eq := <{
+  fun eq : (Type_Num -> Type_Num -> Type_Bool) =>
+    fun m : Type_Num => 
+      fun n : Type_Num => 
+        if m == 0 
+        then n == 0 
+        else 
+          if n == 0 
+          then false 
+          else 
+            eq (n-1) (m-1)
+}>.
+
+Example multistep_fix : 
+<{
+  (fix inner_eq) 1 1
+}> ->>* <{true}>.
+Proof with eauto 8 with zarith local_hints.
+  assert (H_closed_fun_eq : 
+    closed (E_Fix inner_eq)
+  ).
+  {
+    unfold inner_eq.
+    intros x H_n.
+      inversion H_n.
+      inversion H0.
+      inversion H5; subst.
+      inversion H10; subst.
+      inversion H6; subst;
+      try (
+        inversion H1; subst;
+        inversion H4; subst; eauto; fail
+      ).
+      inversion H1; subst; inversion H4; subst; inversion H7; subst; eauto; inversion H9; subst; eauto; inversion H11; subst; eauto.
+  }
+  assert (eq <> n). {
+    intro; inversion H.
+  }
+  assert (eq <> m). {
+    intro; inversion H0.
+  }
+  assert (n <> m). {
+    intro; inversion H1.
+  }
+  assert (closed 1). {
+    intros x Hc; inversion Hc.
+  }
+  assert (closed 0). {
+    intros x Hc; inversion Hc.
+  }
+  eapply multistep_trans.
+  - apply multistep_step. repeat apply ST_App_Left.
+    apply ST_Fix_Fun.
+    repeat apply S_Fun_Neq... 
+    repeat apply S_If...
+  - eapply multistep_trans.
+    + apply multistep_step. apply ST_App_Left.
+      apply ST_App_Fun;
+      try apply S_Fun_Neq;
+      repeat apply S_If...
+    + eapply multistep_trans.
+      * apply multistep_step. apply ST_App_Fun...
+        repeat apply S_If...
+      * {
+      eapply multistep_trans.
+      - apply multistep_step. apply ST_If...
+      - eapply multistep_trans.  
+        + apply multistep_step. apply ST_If_False.
+        + eapply multistep_trans.  
+          * apply multistep_step. apply ST_If...
+          * {
+            eapply multistep_trans.
+            - apply multistep_step. apply ST_If_False...
+            - eapply multistep_trans.
+              + apply multistep_step. repeat apply ST_App_Left.
+                apply ST_Fix_Fun.
+                repeat apply S_Fun_Neq... 
+                repeat apply S_If...
+              + eapply multistep_trans.
+                * apply multistep_step. apply ST_App_Left.
+                  apply ST_App_Right...
+                * {
+                  eapply multistep_trans.
+                  - apply multistep_step. apply ST_App_Left.
+                    simpl.
+                    apply ST_App_Fun...
+                    apply S_Fun_Neq...
+                    repeat apply S_If...
+                  - eapply multistep_trans.
+                    + apply multistep_step. apply ST_App_Right...
+                    + simpl.
+                      eapply multistep_trans.
+                      * apply multistep_step. 
+                        eapply ST_App_Fun...
+                        repeat apply S_If...
+                      * {
+                      eapply multistep_trans.
+                      - apply multistep_step...
+                      - eapply multistep_trans... 
+                      }
+                      
+                }
+          } 
+      
+
+      }
+Qed.
