src/Preservation.v
@@ -14,36 +14,11 @@ Import Maps.Notations.
 
 
 
-(* Theorem preservation : ∀ e e' t,
-  has_type empty e t  ->
-  step e e'  ->
-  has_type empty e' t.
-Proof.
-  (* remember empty as Γ. *)
-  (* induction e;
-  intros * H_type_e H_step.
-  - inversion H_type_e. discriminate H1.
-  - inversion H_type_e; subst. 
-    inversion H_step; subst; eauto with local_hints.
-    inversion H4; subst.
-    eapply Step.subst_typing; eauto.
-  -   *)
-
-  induction e; intros e' τ H_type H_step;
-  try (inversion H_type; subst; 
-    inversion H_step; subst;
-    eauto with local_hints).
-  try (inversion H1; subst; auto; fail). 
-    - inversion H4. eauto with local_hints.
-    -eauto with local_hints.
-
-    
-Qed. *)
 
 Theorem preservation : ∀ e e' t,
-  has_type empty e t  ->
-  step e e'  ->
-  has_type empty e' t.
+  empty ⊢ e ∈ t  ->
+  e ->> e'  ->
+  empty ⊢ e' ∈ t.
 Proof.
   intros * H_type_e. 
   generalize dependent e'.
