src/Types.v
@@ -9,99 +9,103 @@ Definition empty := @Maps.empty type.
 
 
 
+Reserved Notation "Γ '⊢' e '∈' τ" (at level 70, right associativity).
 
 Inductive has_type : context -> expr -> type -> Prop := 
   (* Base λ-calculus *)
   | T_Var: 
       ∀ Γ x t, 
       Γ ? x = Some t -> 
-      has_type Γ (E_Var x) t
+      (Γ ⊢ (E_Var x) ∈ t)
 
   | T_Fun: 
-      ∀ Γ x t1 e t2,
-      has_type (x |-> t1; Γ) e t2 ->
-      has_type Γ (E_Fun x t1 e) (Type_Fun t1 t2)
+      ∀ Γ x t1 e (t2 : type),
+      (x |-> t1; Γ) ⊢ e ∈ t2 ->
+      Γ ⊢ (E_Fun x t1 e) ∈ (Type_Fun t1 t2)
 
   | T_App: 
       ∀ Γ e1 e2 t1 t2, 
-      has_type Γ e2 t1 -> 
-      has_type Γ e1 (Type_Fun t1 t2) ->
-      has_type Γ (E_App e1 e2) t2
+      Γ ⊢ e2 ∈ t1 -> 
+      Γ ⊢ e1 ∈ (Type_Fun t1 t2) ->
+      Γ ⊢ (E_App e1 e2) ∈ t2
 
   (* Booleans and conditions *)
   | T_True: 
       ∀ Γ, 
-      has_type Γ E_True Type_Bool
+      Γ ⊢ E_True ∈ Type_Bool
               
   | T_False: 
       ∀ Γ, 
-      has_type Γ E_False Type_Bool
+      Γ ⊢ E_False ∈ Type_Bool
 
   | T_If: 
       ∀ Γ e1 e2 e3 t, 
-      has_type Γ e1 Type_Bool -> 
-      has_type Γ e2 t -> 
-      has_type Γ e3 t -> 
-      has_type Γ (E_If e1 e2 e3) t 
+      Γ ⊢ e1 ∈ Type_Bool -> 
+      Γ ⊢ e2 ∈ t -> 
+      Γ ⊢ e3 ∈ t -> 
+      Γ ⊢ (E_If e1 e2 e3) ∈ t 
 
   (* Let expressions *)
   | T_Let : 
       ∀ Γ x e1 e2 t1 t2, 
-      has_type Γ e1 t1 -> 
-      has_type (x |-> t1; Γ) e2 t2 -> 
-      has_type Γ (E_Let x e1 e2) t2
+      Γ ⊢ e1 ∈ t1 -> 
+      (x |-> t1; Γ) ⊢ e2 ∈ t2 -> 
+      Γ ⊢ (E_Let x e1 e2) ∈ t2
 
   (* Arithmetic *)
   | T_Num : 
       ∀ Γ z, 
-      has_type Γ (E_Num z) Type_Num 
+      Γ ⊢ (E_Num z) ∈ Type_Num 
 
   | T_Minus : 
       ∀ Γ e1 e2, 
-      has_type Γ e1 Type_Num ->
-      has_type Γ e2 Type_Num ->
-      has_type Γ (E_Minus e1 e2) Type_Num 
+      Γ ⊢ e1 ∈ Type_Num ->
+      Γ ⊢ e2 ∈ Type_Num ->
+      Γ ⊢ (E_Minus e1 e2) ∈ Type_Num 
     
   | T_Eq :
       ∀ Γ e1 e2, 
-      has_type Γ e1 Type_Num ->
-      has_type Γ e2 Type_Num ->
-      has_type Γ (E_Eq e1 e2) Type_Bool 
+      Γ ⊢ e1 ∈ Type_Num ->
+      Γ ⊢ e2 ∈ Type_Num ->
+      Γ ⊢ (E_Eq e1 e2) ∈ Type_Bool 
 
   (* Pairs *)
   | T_Pair :
       ∀ Γ e₁ e₂ t₁ t₂, 
-      has_type Γ e₁ t₁ ->
-      has_type Γ e₂ t₂ ->
-      has_type Γ (E_Pair e₁ e₂) (Type_Prod t₁ t₂) 
+      Γ ⊢ e₁ ∈ t₁ ->
+      Γ ⊢ e₂ ∈ t₂ ->
+      Γ ⊢ (E_Pair e₁ e₂) ∈ (Type_Prod t₁ t₂) 
   | T_First :
       ∀ Γ e t₁ t₂,
-      has_type Γ e (Type_Prod t₁ t₂) ->
-      has_type Γ (E_First e) t₁
+      Γ ⊢ e ∈ (Type_Prod t₁ t₂) ->
+      Γ ⊢ (E_First e) ∈ t₁
   | T_Second :
       ∀ Γ e t₁ t₂,
-      has_type Γ e (Type_Prod t₁ t₂) ->
-      has_type Γ (E_Second e) t₂
+      Γ ⊢ e ∈ (Type_Prod t₁ t₂) ->
+      Γ ⊢ (E_Second e) ∈ t₂
 
   (* Records *)
   | T_Record_Nil :
-      ∀ Γ, has_type Γ E_Record_Nil Type_Record_Nil
+      ∀ Γ, 
+      Γ ⊢ E_Record_Nil ∈ Type_Record_Nil
   | T_Record_Cons :
       ∀ Γ x e tail t_e t_tail, 
-      has_type Γ e t_e -> 
-      has_type Γ tail t_tail -> 
+      Γ ⊢ e ∈ t_e -> 
+      Γ ⊢ tail ∈ t_tail -> 
       record_type t_tail -> 
-      has_type Γ (E_Record_Cons x e tail) (Type_Record_Cons x t_e t_tail) 
+      Γ ⊢ (E_Record_Cons x e tail) ∈ (Type_Record_Cons x t_e t_tail) 
   | T_Record_Access :
       ∀ Γ x e t_e t_acc, 
-      has_type Γ e t_e -> 
+      Γ ⊢ e ∈ t_e -> 
       lookup_type_record x t_e = Some t_acc ->
-      has_type Γ (E_Record_Access e x) t_acc
+      Γ ⊢ (E_Record_Access e x) ∈ t_acc
   
   | T_Fix :
       ∀ Γ e t, 
-      has_type Γ e (Type_Fun t t) -> 
-      has_type Γ (E_Fix e) t
+      Γ ⊢ e ∈ (Type_Fun t t) -> 
+      Γ ⊢ (E_Fix e) ∈ t
+  where
+    "Γ '⊢' e '∈' τ" := (has_type Γ e τ)
 .
 
 Hint Constructors has_type : local_hints.
@@ -110,8 +114,8 @@ Hint Constructors has_type : local_hints.
   
 Local Lemma weakening : ∀ Γ Γ' e t, 
   Maps.includedin Γ Γ' ->
-  has_type Γ e t ->
-  has_type Γ' e t.
+  Γ ⊢ e ∈ t ->
+  Γ' ⊢ e ∈ t.
 Proof.
   intros * H_included H_type.
   generalize dependent Γ'.
@@ -128,11 +132,11 @@ Hint Resolve weakening : local_hints.
 
 
 Local Lemma weakening_empty : ∀ Γ e t, 
-  has_type empty e t ->
-  has_type Γ e t.
+  empty ⊢ e ∈ t ->
+  Γ ⊢ e ∈ t.
 Proof.
-intros. apply (weakening empty); auto.
-intros x v contra. discriminate contra.
+  intros. apply (weakening empty); auto.
+  intros x v contra. discriminate contra.
 Qed.
 
 Hint Resolve weakening_empty : local_hints.
